<?xml version="1.0"?>
<rdf:RDF xmlns="http://www.opensensemap.org/SENPH#"
     xml:base="http://www.opensensemap.org/SENPH"
     xmlns:dc="http://purl.org/dc/elements/1.1/"
     xmlns:ns="http://www.w3.org/2003/06/sw-vocab-status/ns#"
     xmlns:owl="http://www.w3.org/2002/07/owl#"
     xmlns:rdf="http://www.w3.org/1999/02/22-rdf-syntax-ns#"
     xmlns:uo5="http://purl.obolibrary.org/obo/uo5.owl"
     xmlns:wot="http://xmlns.com/wot/0.1/"
     xmlns:xml="http://www.w3.org/XML/1998/namespace"
     xmlns:xsd="http://www.w3.org/2001/XMLSchema#"
     xmlns:rdfs="http://www.w3.org/2000/01/rdf-schema#"
     xmlns:SENPH="http://www.opensensemap.org/SENPH#">
    <owl:Ontology rdf:about="http://www.opensensemap.org/SENPH">
        <owl:imports rdf:resource="http://purl.obolibrary.org/obo/uo5.owl"/>
    </owl:Ontology>
    


    <!-- 
    ///////////////////////////////////////////////////////////////////////////////////////
    //
    // Object Properties
    //
    ///////////////////////////////////////////////////////////////////////////////////////
     -->

    


    <!-- http://www.opensensemap.org/SENPH#canMeasure -->

    <owl:ObjectProperty rdf:about="http://www.opensensemap.org/SENPH#canMeasure">
        <owl:inverseOf rdf:resource="http://www.opensensemap.org/SENPH#measurableBy"/>
        <rdf:type rdf:resource="http://www.w3.org/2002/07/owl#FunctionalProperty"/>
        <rdfs:domain rdf:resource="http://www.opensensemap.org/SENPH#sensorElement"/>
        <rdfs:range rdf:resource="http://www.opensensemap.org/SENPH#phenomenon"/>
        <rdfs:comment xml:lang="en">Relation between a sensor element and a phenomenon, that determines the ability of a sensor element to detect the phenomenon.</rdfs:comment>
        <rdfs:label xml:lang="en">can measure</rdfs:label>
    </owl:ObjectProperty>
    


    <!-- http://www.opensensemap.org/SENPH#describedBy -->

    <owl:ObjectProperty rdf:about="http://www.opensensemap.org/SENPH#describedBy">
        <rdfs:domain rdf:resource="http://www.opensensemap.org/SENPH#phenomenon"/>
        <rdfs:range rdf:resource="http://purl.obolibrary.org/obo/UO_0000000"/>
        <rdfs:comment xml:lang="en">Relation that connects a phenomenon with the units it can described in.</rdfs:comment>
        <rdfs:label xml:lang="en">described by unit</rdfs:label>
    </owl:ObjectProperty>
    


    <!-- http://www.opensensemap.org/SENPH#hasAccuracyUnit -->

    <owl:ObjectProperty rdf:about="http://www.opensensemap.org/SENPH#hasAccuracyUnit">
        <rdfs:domain rdf:resource="http://www.opensensemap.org/SENPH#sensorElement"/>
        <rdfs:range rdf:resource="http://purl.obolibrary.org/obo/UO_0000000"/>
        <rdfs:comment xml:lang="en">Describes the unit in that the accuracy of a sensor element is given.</rdfs:comment>
        <rdfs:label xml:lang="en">has unit of accuracy value</rdfs:label>
    </owl:ObjectProperty>
    


    <!-- http://www.opensensemap.org/SENPH#hasDomain -->

    <owl:ObjectProperty rdf:about="http://www.opensensemap.org/SENPH#hasDomain">
        <owl:inverseOf rdf:resource="http://www.opensensemap.org/SENPH#isDomainOf"/>
        <rdfs:domain rdf:resource="http://www.opensensemap.org/SENPH#phenomenon"/>
        <rdfs:range rdf:resource="http://www.opensensemap.org/SENPH#domain"/>
        <rdfs:comment xml:lang="en">Describes the relation of a phenomenon to a domain it describes some characteristic of.</rdfs:comment>
        <rdfs:label xml:lang="en">has domain</rdfs:label>
    </owl:ObjectProperty>
    


    <!-- http://www.opensensemap.org/SENPH#hasElement -->

    <owl:ObjectProperty rdf:about="http://www.opensensemap.org/SENPH#hasElement">
        <rdfs:subPropertyOf rdf:resource="http://www.w3.org/2002/07/owl#topObjectProperty"/>
        <owl:inverseOf rdf:resource="http://www.opensensemap.org/SENPH#isElementOf"/>
        <rdfs:domain rdf:resource="http://www.opensensemap.org/SENPH#sensor"/>
        <rdfs:range rdf:resource="http://www.opensensemap.org/SENPH#sensorElement"/>
        <rdfs:comment xml:lang="en">Describes the relation between a entity of sensor and its sensor elements</rdfs:comment>
        <rdfs:label xml:lang="en">has element</rdfs:label>
    </owl:ObjectProperty>
    


    <!-- http://www.opensensemap.org/SENPH#hasSensor -->

    <owl:ObjectProperty rdf:about="http://www.opensensemap.org/SENPH#hasSensor">
        <rdfs:subPropertyOf rdf:resource="http://www.w3.org/2002/07/owl#topObjectProperty"/>
        <owl:inverseOf rdf:resource="http://www.opensensemap.org/SENPH#isSensorOf"/>
        <rdfs:domain rdf:resource="http://www.opensensemap.org/SENPH#device"/>
        <rdfs:range rdf:resource="http://www.opensensemap.org/SENPH#sensor"/>
        <rdfs:comment xml:lang="en">Describes the relation between a entity of device and its physical components sensors</rdfs:comment>
        <rdfs:label xml:lang="en">has sensor</rdfs:label>
    </owl:ObjectProperty>
    


    <!-- http://www.opensensemap.org/SENPH#isDomainOf -->

    <owl:ObjectProperty rdf:about="http://www.opensensemap.org/SENPH#isDomainOf">
        <rdfs:comment xml:lang="en">Describes the relation of a domain to the phenomena it is described by.</rdfs:comment>
        <rdfs:label xml:lang="en">is Domain of</rdfs:label>
    </owl:ObjectProperty>
    


    <!-- http://www.opensensemap.org/SENPH#isElementOf -->

    <owl:ObjectProperty rdf:about="http://www.opensensemap.org/SENPH#isElementOf">
        <rdfs:subPropertyOf rdf:resource="http://www.w3.org/2002/07/owl#topObjectProperty"/>
        <rdfs:comment xml:lang="en">Describes the relation between a physical component of kind sensor element and the hosting sensor.</rdfs:comment>
        <rdfs:label xml:lang="en">is element of</rdfs:label>
    </owl:ObjectProperty>
    


    <!-- http://www.opensensemap.org/SENPH#isSensorOf -->

    <owl:ObjectProperty rdf:about="http://www.opensensemap.org/SENPH#isSensorOf">
        <rdfs:subPropertyOf rdf:resource="http://www.w3.org/2002/07/owl#topObjectProperty"/>
        <rdfs:comment xml:lang="en">Describes the relation between a physical component of kind sensor  and the hosting device.</rdfs:comment>
        <rdfs:label xml:lang="en">is sensor of</rdfs:label>
    </owl:ObjectProperty>
    


    <!-- http://www.opensensemap.org/SENPH#measurableBy -->

    <owl:ObjectProperty rdf:about="http://www.opensensemap.org/SENPH#measurableBy">
        <rdfs:comment xml:lang="en">Relation between a phenomenon and a sensor element, that describes by which sensor elements the phenomena can be measured.</rdfs:comment>
        <rdfs:label xml:lang="en">measurable by</rdfs:label>
    </owl:ObjectProperty>
    


    <!-- 
    ///////////////////////////////////////////////////////////////////////////////////////
    //
    // Data properties
    //
    ///////////////////////////////////////////////////////////////////////////////////////
     -->

    


    <!-- http://www.opensensemap.org/SENPH#accuracyValue -->

    <owl:DatatypeProperty rdf:about="http://www.opensensemap.org/SENPH#accuracyValue">
        <rdf:type rdf:resource="http://www.w3.org/2002/07/owl#FunctionalProperty"/>
        <rdfs:domain rdf:resource="http://www.opensensemap.org/SENPH#sensorElement"/>
        <rdfs:range rdf:resource="http://www.w3.org/2001/XMLSchema#float"/>
        <rdfs:comment xml:lang="en">The plus minus value of accuracy of a sensor&apos;s sensor element.</rdfs:comment>
        <rdfs:label xml:lang="en">Value of Accuracy</rdfs:label>
    </owl:DatatypeProperty>
    


    <!-- http://www.opensensemap.org/SENPH#dataSheet -->

    <owl:DatatypeProperty rdf:about="http://www.opensensemap.org/SENPH#dataSheet">
        <rdf:type rdf:resource="http://www.w3.org/2002/07/owl#FunctionalProperty"/>
        <rdfs:domain rdf:resource="http://www.opensensemap.org/SENPH#sensor"/>
        <rdfs:range rdf:resource="http://www.w3.org/2001/XMLSchema#string"/>
        <rdfs:comment xml:lang="en">The URL to the data sheet of a sensor.</rdfs:comment>
        <rdfs:label xml:lang="en">Data Sheet</rdfs:label>
    </owl:DatatypeProperty>
    


    <!-- http://www.opensensemap.org/SENPH#hasContact -->

    <owl:DatatypeProperty rdf:about="http://www.opensensemap.org/SENPH#hasContact">
        <rdfs:domain rdf:resource="http://www.opensensemap.org/SENPH#device"/>
        <rdfs:range rdf:resource="http://www.w3.org/2001/XMLSchema#string"/>
        <rdfs:comment xml:lang="en">A relation that connects a device with an individual (for example person, institution or company), who is the maintainer or developer of the device.</rdfs:comment>
        <rdfs:label xml:lang="en">has contact</rdfs:label>
    </owl:DatatypeProperty>
    


    <!-- http://www.opensensemap.org/SENPH#image -->

    <owl:DatatypeProperty rdf:about="http://www.opensensemap.org/SENPH#image">
        <rdf:type rdf:resource="http://www.w3.org/2002/07/owl#FunctionalProperty"/>
        <rdfs:domain rdf:resource="http://www.opensensemap.org/SENPH#device"/>
        <rdfs:domain rdf:resource="http://www.opensensemap.org/SENPH#sensor"/>
        <rdfs:range rdf:resource="http://www.w3.org/2001/XMLSchema#string"/>
        <rdfs:comment xml:lang="en">The URL to an images of the sensor. Ideally an illustration instead of a photography.</rdfs:comment>
        <rdfs:label xml:lang="en">Image</rdfs:label>
    </owl:DatatypeProperty>
    


    <!-- http://www.opensensemap.org/SENPH#isValid -->

    <owl:DatatypeProperty rdf:about="http://www.opensensemap.org/SENPH#isValid">
        <rdfs:range rdf:resource="http://www.w3.org/2001/XMLSchema#boolean"/>
    </owl:DatatypeProperty>
    


    <!-- http://www.opensensemap.org/SENPH#lifePeriod -->

    <owl:DatatypeProperty rdf:about="http://www.opensensemap.org/SENPH#lifePeriod">
        <rdf:type rdf:resource="http://www.w3.org/2002/07/owl#FunctionalProperty"/>
        <rdfs:domain rdf:resource="http://www.opensensemap.org/SENPH#sensor"/>
        <rdfs:range rdf:resource="http://www.w3.org/2001/XMLSchema#dateTime"/>
        <rdfs:comment xml:lang="en">The average life period of a sensor. Typically given by the manufacturer of a sensor.</rdfs:comment>
        <rdfs:label xml:lang="en">Life period</rdfs:label>
    </owl:DatatypeProperty>
    


    <!-- http://www.opensensemap.org/SENPH#manufacturer -->

    <owl:DatatypeProperty rdf:about="http://www.opensensemap.org/SENPH#manufacturer">
        <rdfs:domain rdf:resource="http://www.opensensemap.org/SENPH#sensor"/>
        <rdfs:range rdf:resource="http://www.w3.org/2001/XMLSchema#string"/>
        <rdfs:comment xml:lang="en">The manufacturer of a sensor.</rdfs:comment>
        <rdfs:label xml:lang="en">Manufacturer</rdfs:label>
    </owl:DatatypeProperty>
    


    <!-- http://www.opensensemap.org/SENPH#priceInEuro -->

    <owl:DatatypeProperty rdf:about="http://www.opensensemap.org/SENPH#priceInEuro">
        <rdf:type rdf:resource="http://www.w3.org/2002/07/owl#FunctionalProperty"/>
        <rdfs:domain rdf:resource="http://www.opensensemap.org/SENPH#sensor"/>
        <rdfs:range rdf:resource="http://www.w3.org/2001/XMLSchema#float"/>
        <rdfs:comment xml:lang="en">Gives the approximate prices of a sensor in Euro, by a float value.</rdfs:comment>
        <rdfs:label xml:lang="en">Price in Euro</rdfs:label>
    </owl:DatatypeProperty>
    


    <!-- http://www.opensensemap.org/SENPH#website -->

    <owl:DatatypeProperty rdf:about="http://www.opensensemap.org/SENPH#website">
        <rdfs:domain rdf:resource="http://www.opensensemap.org/SENPH#device"/>
        <rdfs:range rdf:resource="http://www.w3.org/2001/XMLSchema#string"/>
        <rdfs:comment xml:lang="en">The website of the devices&apos; project, maintainer, developer or contact person.</rdfs:comment>
        <rdfs:label xml:lang="en">Website</rdfs:label>
    </owl:DatatypeProperty>
    


    <!-- 
    ///////////////////////////////////////////////////////////////////////////////////////
    //
    // Classes
    //
    ///////////////////////////////////////////////////////////////////////////////////////
     -->

    


    <!-- http://www.opensensemap.org/SENPH#HDC1080 -->

    <owl:Class rdf:about="http://www.opensensemap.org/SENPH#HDC1080">
        <rdfs:subClassOf rdf:resource="http://www.opensensemap.org/SENPH#sensor"/>
    </owl:Class>
    


    <!-- http://www.opensensemap.org/SENPH#airTemperature -->

    <owl:Class rdf:about="http://www.opensensemap.org/SENPH#airTemperature">
        <rdfs:subClassOf rdf:resource="http://www.opensensemap.org/SENPH#temperature"/>
    </owl:Class>
    


    <!-- http://www.opensensemap.org/SENPH#climatePhenomena -->

    <owl:Class rdf:about="http://www.opensensemap.org/SENPH#climatePhenomena">
        <rdfs:subClassOf rdf:resource="http://www.opensensemap.org/SENPH#domain"/>
        <rdfs:subClassOf>
            <owl:Restriction>
                <owl:onProperty rdf:resource="http://www.opensensemap.org/SENPH#isDomainOf"/>
                <owl:someValuesFrom rdf:resource="http://www.opensensemap.org/SENPH#temperature"/>
            </owl:Restriction>
        </rdfs:subClassOf>
    </owl:Class>
    


    <!-- http://www.opensensemap.org/SENPH#device -->

    <owl:Class rdf:about="http://www.opensensemap.org/SENPH#device">
        <rdfs:subClassOf>
            <owl:Restriction>
                <owl:onProperty rdf:resource="http://www.opensensemap.org/SENPH#hasSensor"/>
                <owl:someValuesFrom rdf:resource="http://www.opensensemap.org/SENPH#sensor"/>
            </owl:Restriction>
        </rdfs:subClassOf>
        <rdfs:subClassOf>
            <owl:Restriction>
                <owl:onProperty rdf:resource="http://www.opensensemap.org/SENPH#isValid"/>
                <owl:qualifiedCardinality rdf:datatype="http://www.w3.org/2001/XMLSchema#nonNegativeInteger">1</owl:qualifiedCardinality>
                <owl:onDataRange rdf:resource="http://www.w3.org/2001/XMLSchema#boolean"/>
            </owl:Restriction>
        </rdfs:subClassOf>
        <rdfs:subClassOf>
            <owl:Restriction>
                <owl:onProperty rdf:resource="http://www.opensensemap.org/SENPH#website"/>
                <owl:maxQualifiedCardinality rdf:datatype="http://www.w3.org/2001/XMLSchema#nonNegativeInteger">1</owl:maxQualifiedCardinality>
                <owl:onDataRange rdf:resource="http://www.w3.org/2001/XMLSchema#string"/>
            </owl:Restriction>
        </rdfs:subClassOf>
    </owl:Class>
    


    <!-- http://www.opensensemap.org/SENPH#domain -->

    <owl:Class rdf:about="http://www.opensensemap.org/SENPH#domain">
        <rdfs:subClassOf>
            <owl:Restriction>
                <owl:onProperty rdf:resource="http://www.opensensemap.org/SENPH#isDomainOf"/>
                <owl:someValuesFrom rdf:resource="http://www.opensensemap.org/SENPH#phenomenon"/>
            </owl:Restriction>
        </rdfs:subClassOf>
        <rdfs:subClassOf>
            <owl:Restriction>
                <owl:onProperty rdf:resource="http://www.opensensemap.org/SENPH#isValid"/>
                <owl:qualifiedCardinality rdf:datatype="http://www.w3.org/2001/XMLSchema#nonNegativeInteger">1</owl:qualifiedCardinality>
                <owl:onDataRange rdf:resource="http://www.w3.org/2001/XMLSchema#boolean"/>
            </owl:Restriction>
        </rdfs:subClassOf>
    </owl:Class>
    


    <!-- http://www.opensensemap.org/SENPH#phenomenon -->

    <owl:Class rdf:about="http://www.opensensemap.org/SENPH#phenomenon">
        <rdfs:subClassOf>
            <owl:Restriction>
                <owl:onProperty rdf:resource="http://www.opensensemap.org/SENPH#describedBy"/>
                <owl:someValuesFrom rdf:resource="http://purl.obolibrary.org/obo/UO_0000000"/>
            </owl:Restriction>
        </rdfs:subClassOf>
        <rdfs:subClassOf>
            <owl:Restriction>
                <owl:onProperty rdf:resource="http://www.opensensemap.org/SENPH#isValid"/>
                <owl:qualifiedCardinality rdf:datatype="http://www.w3.org/2001/XMLSchema#nonNegativeInteger">1</owl:qualifiedCardinality>
                <owl:onDataRange rdf:resource="http://www.w3.org/2001/XMLSchema#boolean"/>
            </owl:Restriction>
        </rdfs:subClassOf>
    </owl:Class>
    


    <!-- http://www.opensensemap.org/SENPH#pm10concentration -->

    <owl:Class rdf:about="http://www.opensensemap.org/SENPH#pm10concentration">
        <rdfs:subClassOf rdf:resource="http://www.opensensemap.org/SENPH#phenomenon"/>
    </owl:Class>
    


    <!-- http://www.opensensemap.org/SENPH#relativeHumidity -->

    <owl:Class rdf:about="http://www.opensensemap.org/SENPH#relativeHumidity">
        <rdfs:subClassOf rdf:resource="http://www.opensensemap.org/SENPH#phenomenon"/>
    </owl:Class>
    


    <!-- http://www.opensensemap.org/SENPH#sensor -->

    <owl:Class rdf:about="http://www.opensensemap.org/SENPH#sensor">
        <rdfs:subClassOf>
            <owl:Restriction>
                <owl:onProperty rdf:resource="http://www.opensensemap.org/SENPH#hasElement"/>
                <owl:someValuesFrom rdf:resource="http://www.opensensemap.org/SENPH#sensorElement"/>
            </owl:Restriction>
        </rdfs:subClassOf>
        <rdfs:subClassOf>
            <owl:Restriction>
                <owl:onProperty rdf:resource="http://www.opensensemap.org/SENPH#manufacturer"/>
                <owl:someValuesFrom rdf:resource="http://www.w3.org/2001/XMLSchema#string"/>
            </owl:Restriction>
        </rdfs:subClassOf>
        <rdfs:subClassOf>
            <owl:Restriction>
                <owl:onProperty rdf:resource="http://www.opensensemap.org/SENPH#isValid"/>
                <owl:qualifiedCardinality rdf:datatype="http://www.w3.org/2001/XMLSchema#nonNegativeInteger">1</owl:qualifiedCardinality>
                <owl:onDataRange rdf:resource="http://www.w3.org/2001/XMLSchema#boolean"/>
            </owl:Restriction>
        </rdfs:subClassOf>
        <rdfs:subClassOf>
            <owl:Restriction>
                <owl:onProperty rdf:resource="http://www.opensensemap.org/SENPH#dataSheet"/>
                <owl:maxQualifiedCardinality rdf:datatype="http://www.w3.org/2001/XMLSchema#nonNegativeInteger">1</owl:maxQualifiedCardinality>
                <owl:onDataRange rdf:resource="http://www.w3.org/2001/XMLSchema#string"/>
            </owl:Restriction>
        </rdfs:subClassOf>
        <rdfs:subClassOf>
            <owl:Restriction>
                <owl:onProperty rdf:resource="http://www.opensensemap.org/SENPH#lifePeriod"/>
                <owl:maxQualifiedCardinality rdf:datatype="http://www.w3.org/2001/XMLSchema#nonNegativeInteger">1</owl:maxQualifiedCardinality>
                <owl:onDataRange rdf:resource="http://www.w3.org/2001/XMLSchema#string"/>
            </owl:Restriction>
        </rdfs:subClassOf>
        <rdfs:subClassOf>
            <owl:Restriction>
                <owl:onProperty rdf:resource="http://www.opensensemap.org/SENPH#priceInEuro"/>
                <owl:maxQualifiedCardinality rdf:datatype="http://www.w3.org/2001/XMLSchema#nonNegativeInteger">1</owl:maxQualifiedCardinality>
                <owl:onDataRange rdf:resource="http://www.w3.org/2001/XMLSchema#string"/>
            </owl:Restriction>
        </rdfs:subClassOf>
    </owl:Class>
    


    <!-- http://www.opensensemap.org/SENPH#sensorElement -->

    <owl:Class rdf:about="http://www.opensensemap.org/SENPH#sensorElement">
        <rdfs:subClassOf>
            <owl:Restriction>
                <owl:onProperty rdf:resource="http://www.opensensemap.org/SENPH#canMeasure"/>
                <owl:qualifiedCardinality rdf:datatype="http://www.w3.org/2001/XMLSchema#nonNegativeInteger">1</owl:qualifiedCardinality>
                <owl:onClass rdf:resource="http://www.opensensemap.org/SENPH#phenomenon"/>
            </owl:Restriction>
        </rdfs:subClassOf>
        <rdfs:subClassOf>
            <owl:Restriction>
                <owl:onProperty rdf:resource="http://www.opensensemap.org/SENPH#hasAccuracyUnit"/>
                <owl:qualifiedCardinality rdf:datatype="http://www.w3.org/2001/XMLSchema#nonNegativeInteger">1</owl:qualifiedCardinality>
                <owl:onClass rdf:resource="http://purl.obolibrary.org/obo/UO_0000000"/>
            </owl:Restriction>
        </rdfs:subClassOf>
        <rdfs:subClassOf>
            <owl:Restriction>
                <owl:onProperty rdf:resource="http://www.opensensemap.org/SENPH#isElementOf"/>
                <owl:qualifiedCardinality rdf:datatype="http://www.w3.org/2001/XMLSchema#nonNegativeInteger">1</owl:qualifiedCardinality>
                <owl:onClass rdf:resource="http://www.opensensemap.org/SENPH#sensor"/>
            </owl:Restriction>
        </rdfs:subClassOf>
        <rdfs:subClassOf>
            <owl:Restriction>
                <owl:onProperty rdf:resource="http://www.opensensemap.org/SENPH#isValid"/>
                <owl:qualifiedCardinality rdf:datatype="http://www.w3.org/2001/XMLSchema#nonNegativeInteger">1</owl:qualifiedCardinality>
                <owl:onDataRange rdf:resource="http://www.w3.org/2001/XMLSchema#boolean"/>
            </owl:Restriction>
        </rdfs:subClassOf>
    </owl:Class>
    


    <!-- http://www.opensensemap.org/SENPH#temperature -->

    <owl:Class rdf:about="http://www.opensensemap.org/SENPH#temperature">
        <rdfs:subClassOf rdf:resource="http://www.opensensemap.org/SENPH#phenomenon"/>
        <rdfs:subClassOf>
            <owl:Restriction>
                <owl:onProperty rdf:resource="http://www.opensensemap.org/SENPH#describedBy"/>
                <owl:allValuesFrom rdf:resource="http://purl.obolibrary.org/obo/UO_0000005"/>
            </owl:Restriction>
        </rdfs:subClassOf>
    </owl:Class>
    


    <!-- http://www.opensensemap.org/SENPH#waterTemperature -->

    <owl:Class rdf:about="http://www.opensensemap.org/SENPH#waterTemperature">
        <rdfs:subClassOf rdf:resource="http://www.opensensemap.org/SENPH#temperature"/>
    </owl:Class>
    


    <!-- http://www.opensensemap.org/SENPH#sensebox:home -->

    <owl:Class rdf:about="http://www.opensensemap.org/SENPH#sensebox:home">
        <rdfs:subClassOf rdf:resource="http://www.opensensemap.org/SENPH#device"/>
        <rdfs:subClassOf>
            <owl:Restriction>
                <owl:onProperty rdf:resource="http://www.opensensemap.org/SENPH#hasSensor"/>
                <owl:someValuesFrom rdf:resource="http://www.opensensemap.org/SENPH#HDC1080"/>
            </owl:Restriction>
        </rdfs:subClassOf>
    </owl:Class>
    


    <!-- 
    ///////////////////////////////////////////////////////////////////////////////////////
    //
    // Individuals
    //
    ///////////////////////////////////////////////////////////////////////////////////////
     -->

    


    <!-- http://www.opensensemap.org/SENPH#HDC1080 -->

    <owl:NamedIndividual rdf:about="http://www.opensensemap.org/SENPH#HDC1080">
        <hasElement rdf:resource="http://www.opensensemap.org/SENPH#humi_HDC1080"/>
        <hasElement rdf:resource="http://www.opensensemap.org/SENPH#temp_HDC1080"/>
    </owl:NamedIndividual>
    


    <!-- http://www.opensensemap.org/SENPH#airTemperature -->

    <owl:NamedIndividual rdf:about="http://www.opensensemap.org/SENPH#airTemperature">
        <describedBy rdf:resource="http://purl.obolibrary.org/obo/UO_0000012"/>
        <measurableBy rdf:resource="http://www.opensensemap.org/SENPH#temp_HDC1080"/>
    </owl:NamedIndividual>
    


    <!-- http://www.opensensemap.org/SENPH#climatePhenomena -->

    <owl:NamedIndividual rdf:about="http://www.opensensemap.org/SENPH#climatePhenomena">
        <isDomainOf rdf:resource="http://www.opensensemap.org/SENPH#relativeHumidity"/>
        <isDomainOf rdf:resource="http://www.opensensemap.org/SENPH#temperature"/>
    </owl:NamedIndividual>
    


    <!-- http://www.opensensemap.org/SENPH#device -->

    <owl:NamedIndividual rdf:about="http://www.opensensemap.org/SENPH#device">
        <hasSensor rdf:resource="http://www.opensensemap.org/SENPH#HDC1080"/>
    </owl:NamedIndividual>
    


    <!-- http://www.opensensemap.org/SENPH#domain -->

    <owl:NamedIndividual rdf:about="http://www.opensensemap.org/SENPH#domain"/>
    


    <!-- http://www.opensensemap.org/SENPH#humi_HDC1080 -->

    <owl:NamedIndividual rdf:about="http://www.opensensemap.org/SENPH#humi_HDC1080"/>
    


    <!-- http://www.opensensemap.org/SENPH#phenomenon -->

    <owl:NamedIndividual rdf:about="http://www.opensensemap.org/SENPH#phenomenon"/>
    


    <!-- http://www.opensensemap.org/SENPH#pm10concentration -->

    <owl:NamedIndividual rdf:about="http://www.opensensemap.org/SENPH#pm10concentration">
        <rdf:type rdf:resource="http://www.opensensemap.org/SENPH#pm10concentration"/>
    </owl:NamedIndividual>
    


    <!-- http://www.opensensemap.org/SENPH#relativeHumidity -->

    <owl:NamedIndividual rdf:about="http://www.opensensemap.org/SENPH#relativeHumidity">
        <measurableBy rdf:resource="http://www.opensensemap.org/SENPH#humi_HDC1080"/>
    </owl:NamedIndividual>
    


    <!-- http://www.opensensemap.org/SENPH#sensor -->

    <owl:NamedIndividual rdf:about="http://www.opensensemap.org/SENPH#sensor"/>
    


    <!-- http://www.opensensemap.org/SENPH#sensorElement -->

    <owl:NamedIndividual rdf:about="http://www.opensensemap.org/SENPH#sensorElement"/>
    


    <!-- http://www.opensensemap.org/SENPH#temp_HDC1080 -->

    <owl:NamedIndividual rdf:about="http://www.opensensemap.org/SENPH#temp_HDC1080"/>
    


    <!-- http://www.opensensemap.org/SENPH#temperature -->

    <owl:NamedIndividual rdf:about="http://www.opensensemap.org/SENPH#temperature"/>
    


    <!-- http://www.opensensemap.org/SENPH#waterTemperature -->

    <owl:NamedIndividual rdf:about="http://www.opensensemap.org/SENPH#waterTemperature">
        <describedBy rdf:resource="http://purl.obolibrary.org/obo/UO_0000012"/>
        <isValid rdf:datatype="http://www.w3.org/2001/XMLSchema#boolean">true</isValid>
    </owl:NamedIndividual>
    


    <!-- http://www.opensensemap.org/SENPH#sensebox:home -->

    <owl:NamedIndividual rdf:about="http://www.opensensemap.org/SENPH#sensebox:home">
        <hasSensor rdf:resource="http://www.opensensemap.org/SENPH#HDC1080"/>
    </owl:NamedIndividual>
    


    <!-- 
    ///////////////////////////////////////////////////////////////////////////////////////
    //
    // Annotations
    //
    ///////////////////////////////////////////////////////////////////////////////////////
     -->

    <rdf:Description rdf:about="http://www.opensensemap.org/SENPH#device">
        <rdfs:comment xml:lang="en">A device is a system that deploys at least one sensor and reads in the values of sensors. It has a physical packing.</rdfs:comment>
        <rdfs:label xml:lang="en">Device</rdfs:label>
    </rdf:Description>
    <rdf:Description rdf:about="http://www.opensensemap.org/SENPH#domain">
        <rdfs:label xml:lang="en">Phenomena Domain</rdfs:label>
        <rdfs:comment xml:lang="en">An abstract collection of phenomena, that are describe a certain domain.</rdfs:comment>
    </rdf:Description>
    <rdf:Description rdf:about="http://www.opensensemap.org/SENPH#phenomenon">
        <rdfs:comment xml:lang="en">An environmental phenomenon is a state or non-human entity that can be observed and measured in the context of environmental monitoring. It has a unique value for a given time and location.</rdfs:comment>
        <rdfs:label xml:lang="en">Environmental Phenomenon</rdfs:label>
    </rdf:Description>
    <rdf:Description rdf:about="http://www.opensensemap.org/SENPH#pm10concentration">
        <rdfs:label xml:lang="en">PM10 concentration</rdfs:label>
    </rdf:Description>
    <rdf:Description rdf:about="http://www.opensensemap.org/SENPH#relativeHumidity">
        <rdfs:label xml:lang="en">relative Humidity</rdfs:label>
    </rdf:Description>
    <rdf:Description rdf:about="http://www.opensensemap.org/SENPH#sensor">
        <rdfs:label xml:lang="en">Sensor</rdfs:label>
        <rdfs:comment xml:lang="en">A sensor element including its physical packaging and external connections (e.g., electrical or
optical).

Council, National R.: Expanding the Vision of Sensor Materials. Washington, DC : The National Academies Press, 1995</rdfs:comment>
    </rdf:Description>
    <rdf:Description rdf:about="http://www.opensensemap.org/SENPH#sensorElement">
        <rdfs:comment xml:lang="en">A sensor element is the part of a sensor that measures a phenomenon. Excluding any other sensor components. There can be several sensor element on one sensor.</rdfs:comment>
        <rdfs:label xml:lang="en">Sensor element</rdfs:label>
        <rdfs:comment xml:lang="en">&quot;The fundamental transduction mechanism (e.g., a material) that converts one form of energy into another. Some sensors may incorporate more than one sensor element (e.g., a compound sensor). &quot;
Council, National R.: Expanding the Vision of Sensor Materials. Washington, DC : The National Academies Press, 1995</rdfs:comment>
    </rdf:Description>
    


    <!-- 
    ///////////////////////////////////////////////////////////////////////////////////////
    //
    // General axioms
    //
    ///////////////////////////////////////////////////////////////////////////////////////
     -->

    <rdf:Description>
        <rdf:type rdf:resource="http://www.w3.org/2002/07/owl#AllDisjointClasses"/>
        <owl:members rdf:parseType="Collection">
            <rdf:Description rdf:about="http://www.opensensemap.org/SENPH#device"/>
            <rdf:Description rdf:about="http://www.opensensemap.org/SENPH#domain"/>
            <rdf:Description rdf:about="http://www.opensensemap.org/SENPH#phenomenon"/>
            <rdf:Description rdf:about="http://www.opensensemap.org/SENPH#sensor"/>
            <rdf:Description rdf:about="http://www.opensensemap.org/SENPH#sensorElement"/>
        </owl:members>
    </rdf:Description>
</rdf:RDF>



<!-- Generated by the OWL API (version 4.5.6.2018-09-06T00:27:41Z) https://github.com/owlcs/owlapi -->

